src/dafny/beacon/Helpers.p.dfy
@@ -1,0 +1,198 @@
+/*
+ * Copyright 2021 ConsenSys Software Inc.
+ *
+ * Licensed under the Apache License, Version 2.0 (the "License"); you may 
+ * not use this file except in compliance with the License. You may obtain 
+ * a copy of the License at http://www.apache.org/licenses/LICENSE-2.0
+ *
+ * Unless required by applicable law or agreed to in writing, software dis-
+ * tributed under the License is distributed on an "AS IS" BASIS, WITHOUT 
+ * WARRANTIES OR CONDITIONS OF ANY KIND, either express or implied. See the 
+ * License for the specific language governing permissions and limitations 
+ * under the License.
+ */
+
+include "../utils/MathHelpers.dfy"
+include "../utils/NativeTypes.dfy"
+
+include "../ssz/Constants.dfy"
+
+/**
+ *  Proofs for misc helpers
+ */
+module BeaconHelperProofs {
+
+    //  Import some constants, types and beacon chain helpers.
+    import opened MathHelpers
+    import opened NativeTypes
+
+    import opened Constants
+    
+    /**
+     *  A proof to  assist with the function method compute_committee
+     *
+     *  @param  len     A positive integer. 
+     *  @param  index   A positive integer. 
+     *  @param  count   A positive integer. 
+     *  @return         A proof that if count > 0, (len * index / count) is a uint64,
+     *                  and (len * (index+1) / count) is a uint64 then 
+     *                  len * (index +1) / count >= len * index  / count.
+     */
+    lemma computeCommitteeLemma(len: nat, index: nat, count: nat)
+        requires count > 0
+        requires len * index / count  < 0x10000000000000000
+        requires len * (index +1) / count < 0x10000000000000000
+        ensures len * (index +1) / count >= len * index  / count
+    {
+        commonDivRule(len * (index +1), len * index, count);
+    }
+
+    /**
+     *  A proof that if len_indices > 2^22 then at least one committee formed will be of a length that breaches 
+     *  the upper bound of MAX_VALIDATORS_PER_COMMITTEE.
+     *
+     *  @param  len_indices     A positive integer representing the number of active validators. 
+     *  @param  CPS             A positive integer representing the number of committees per slot. 
+     *  @return                 A proof that if len_indices > 2^22 then at least one committee formed will be of 
+     *                          a length that breaches the upper bound of MAX_VALIDATORS_PER_COMMITTEE.
+     */
+    lemma proveAtLeastOneCommitteeFormedBreachsBound(len_indices: nat, CPS: nat)
+        requires TWO_UP_11 as nat * TWO_UP_11 as nat < len_indices 
+        requires CPS == max(1, min(MAX_COMMITTEES_PER_SLOT as nat, len_indices/ SLOTS_PER_EPOCH  as nat/ TARGET_COMMITTEE_SIZE as nat) as nat)
+        ensures 
+            exists cIndex, slot  | 0 <= cIndex < CPS && 0 <= slot < SLOTS_PER_EPOCH as nat :: 
+            ((len_indices * ((slot * CPS + cIndex) + 1) / (CPS * SLOTS_PER_EPOCH as nat)) - (len_indices * (slot * CPS + cIndex)  / (CPS * SLOTS_PER_EPOCH as nat)) > MAX_VALIDATORS_PER_COMMITTEE as nat)
+    {
+        assert CPS == 64;
+        
+        assert exists cIndex, slot  | 0 <= cIndex < CPS && 0 <= slot < SLOTS_PER_EPOCH as nat :: 
+               ((len_indices * ((slot * CPS + cIndex) + 1) / (CPS * SLOTS_PER_EPOCH as nat)) - (len_indices * (slot * CPS + cIndex)  / (CPS * SLOTS_PER_EPOCH as nat)) > MAX_VALIDATORS_PER_COMMITTEE as nat)
+               by
+               {
+                    assert 
+                    (len_indices * ((31 * CPS + 63) + 1) / (CPS * SLOTS_PER_EPOCH as nat)) - (len_indices * (31 * CPS + 63)  / (CPS * SLOTS_PER_EPOCH as nat)) > MAX_VALIDATORS_PER_COMMITTEE as nat;
+               }
+    }
+
+    /**
+     *  A proof that if len_indices > 2^22 then at least one committee formed will be of a length that breaches 
+     *  the upper bound of MAX_VALIDATORS_PER_COMMITTEE.
+     *
+     *  @param  len_indices     A positive integer representing the number of active validators. 
+     *  @param  CPS             A positive integer representing the number of committees per slot. 
+     *  @param  slot            A positive integer representing the slot. 
+     *  @param  cIndex          A positive integer representing the committee index. 
+     *  @return                 A proof that if len_indices >= ((2^22) + (2^11)) then all committees formed will be of 
+     *                          a length that breaches the upper bound of MAX_VALIDATORS_PER_COMMITTEE.
+     */
+    lemma proveAllCommitteesFormedBreachBound(len_indices: nat, CPS: nat, slot: nat, cIndex: nat)
+        requires TWO_UP_5 as nat <= len_indices 
+        requires CPS == max(1, min(MAX_COMMITTEES_PER_SLOT as nat, len_indices/ SLOTS_PER_EPOCH  as nat/ TARGET_COMMITTEE_SIZE as nat) as nat)
+        requires 0 <= slot < SLOTS_PER_EPOCH as nat// i.e. slot % SPE
+        requires 0 <= cIndex < CPS
+
+        ensures var start :=  (len_indices * (slot * CPS + cIndex) ) / (CPS * SLOTS_PER_EPOCH as nat);
+                var end := (len_indices * ((slot * CPS + cIndex) + 1)) / (CPS * SLOTS_PER_EPOCH as nat);
+
+                len_indices >= ((TWO_UP_11 * TWO_UP_11) + TWO_UP_11) as nat ==> end - start > MAX_VALIDATORS_PER_COMMITTEE as nat
+                // at this point all committees formed will breach the maximum size bound
+    {
+        var start :=  (len_indices * (slot * CPS + cIndex) ) / (CPS * SLOTS_PER_EPOCH as nat);
+        var end := (len_indices * ((slot * CPS + cIndex) + 1)) / (CPS * SLOTS_PER_EPOCH as nat);
+
+        assert len_indices >= ((TWO_UP_11 * TWO_UP_11) + TWO_UP_11) as nat ==> end - start > MAX_VALIDATORS_PER_COMMITTEE as nat;
+    }
+
+    /**
+     *  A proof that if 32 <= len_indices <= > 2^22 then all committees formed will be of 0 < length <= MAX_VALIDATORS_PER_COMMITTEE.
+     *  i.e. a valid length
+     *
+     *  @param  len_indices     A positive integer representing the number of active validators. 
+     *  @param  CPS             A positive integer representing the number of committees per slot. 
+     *  @param  slot            A positive integer representing the slot. 
+     *  @param  cIndex          A positive integer representing the committee index. 
+     *  @return                 A proof that if 32 <= len_indices <= > 2^22 then all committees formed will be of a valid length.
+     */
+    lemma proveActiveValidatorsSatisfyBounds(len_indices: nat, CPS: nat, slot: nat, cIndex: nat)
+        requires TWO_UP_5 as nat <= len_indices <= TWO_UP_11 as nat * TWO_UP_11 as nat // valid range for the number of active validators
+
+        requires CPS == max(1, min(MAX_COMMITTEES_PER_SLOT as nat, len_indices/ SLOTS_PER_EPOCH  as nat/ TARGET_COMMITTEE_SIZE as nat) as nat)
+        requires 0 <= slot < SLOTS_PER_EPOCH as nat;
+        requires 0 <= cIndex < CPS;
+
+        ensures var start :=  (len_indices * (slot * CPS + cIndex) ) / (CPS * SLOTS_PER_EPOCH as nat);
+                var end := (len_indices * ((slot * CPS + cIndex) + 1)) / (CPS * SLOTS_PER_EPOCH as nat);
+    
+                0 < end - start <= MAX_VALIDATORS_PER_COMMITTEE as nat
+    {
+        var start :=  (len_indices * (slot * CPS + cIndex) ) / (CPS * SLOTS_PER_EPOCH as nat);
+        var end := (len_indices * ((slot * CPS + cIndex) + 1)) / (CPS * SLOTS_PER_EPOCH as nat);
+
+        //assert 63 * SLOTS_PER_EPOCH as nat * TARGET_COMMITTEE_SIZE as nat <= len_indices < 64 * SLOTS_PER_EPOCH as nat * TARGET_COMMITTEE_SIZE as nat ==> CPS == 63;
+        //assert TWO_UP_18 as nat - TWO_UP_12 as nat <= len_indices < TWO_UP_18 as nat ==> CPS == 63;
+
+        assert  TWO_UP_18 as nat <= len_indices ==> CPS == 64;
+        assert TWO_UP_18 as nat <= len_indices <= TWO_UP_11 as nat * TWO_UP_11 as nat && CPS == 64 ==> 0 < end - start <= MAX_VALIDATORS_PER_COMMITTEE as nat;
+
+        assert 63 * SLOTS_PER_EPOCH as nat * TARGET_COMMITTEE_SIZE as nat <= len_indices < TWO_UP_18 as nat && CPS == 63 ==> 0 < end - start <= MAX_VALIDATORS_PER_COMMITTEE as nat;
+
+        //assert 62 * SLOTS_PER_EPOCH as nat * TARGET_COMMITTEE_SIZE as nat <= len_indices < 63 * SLOTS_PER_EPOCH as nat * TARGET_COMMITTEE_SIZE as nat && CPS == 62 ==> 
+        //    0 < (len_indices * ((slot * CPS + cIndex) + 1)) / (CPS * SLOTS_PER_EPOCH as nat) - (len_indices * (slot * CPS + cIndex) ) / (CPS * SLOTS_PER_EPOCH as nat) <= MAX_VALIDATORS_PER_COMMITTEE as nat;
+
+        //assert 61 * SLOTS_PER_EPOCH as nat * TARGET_COMMITTEE_SIZE as nat <= len_indices < 62 * SLOTS_PER_EPOCH as nat * TARGET_COMMITTEE_SIZE as nat && CPS == 61 ==> 
+        //    0 < (len_indices * ((slot * CPS + cIndex) + 1)) / (CPS * SLOTS_PER_EPOCH as nat) - (len_indices * (slot * CPS + cIndex) ) / (CPS * SLOTS_PER_EPOCH as nat) <= MAX_VALIDATORS_PER_COMMITTEE as nat;
+
+        assert forall i :: 2 <= i <= 63 && (i-1) * SLOTS_PER_EPOCH as nat * TARGET_COMMITTEE_SIZE as nat <= len_indices < i * SLOTS_PER_EPOCH as nat * TARGET_COMMITTEE_SIZE as nat ==> CPS == i-1 ;
+        
+        assert forall i :: 2 <= i <= 63 && (i-1) * SLOTS_PER_EPOCH as nat * TARGET_COMMITTEE_SIZE as nat <= len_indices < i * SLOTS_PER_EPOCH as nat * TARGET_COMMITTEE_SIZE as nat && CPS == i-1 ==> 
+            0 < end - start <= MAX_VALIDATORS_PER_COMMITTEE as nat;
+
+
+        assert len_indices < 2 * SLOTS_PER_EPOCH as nat * TARGET_COMMITTEE_SIZE as nat ==> CPS == 1;
+        assert TWO_UP_5 as nat <= len_indices < 2 * SLOTS_PER_EPOCH as nat * TARGET_COMMITTEE_SIZE as nat && CPS == 1 ==> 0 < end - start <= MAX_VALIDATORS_PER_COMMITTEE as nat;
+
+        assert TWO_UP_5 as nat <= len_indices <= TWO_UP_11 as nat * TWO_UP_11 as nat ==> 0 < end - start <= MAX_VALIDATORS_PER_COMMITTEE as nat;
+    
+        //assert TWO_UP_5 as nat <= len_indices <= TWO_UP_11 as nat * TWO_UP_11 as nat && CPS == max(1, min(MAX_COMMITTEES_PER_SLOT as nat, len_indices/ SLOTS_PER_EPOCH  as nat/ TARGET_COMMITTEE_SIZE as nat) as nat) 
+        // ==> 
+         //   0 < (len_indices * ((slot * CPS + cIndex) + 1)) / (CPS * SLOTS_PER_EPOCH as nat) - (len_indices * (slot * CPS + cIndex) ) / (CPS * SLOTS_PER_EPOCH as nat) <= MAX_VALIDATORS_PER_COMMITTEE as nat;
+
+    }
+
+    /**
+     *   A proof to  assist with the function method get_beacon_committee.
+     *
+     *  @param  len_indices     A positive integer representing the number of active validators. 
+     *  @param  CPS             A positive integer representing the number of committees per slot. 
+     *  @param  slot            A positive integer representing the slot. 
+     *  @param  cIndex          A positive integer representing the committee index. 
+     *  @return                 A proof that len_indices * ((slot * CPS + cIndex) + 1) / (CPS * SLOTS_PER_EPOCH as nat) > len_indices * (slot * CPS + cIndex) / (CPS * SLOTS_PER_EPOCH as nat).
+     */
+    lemma getBeaconCommitteeLemma(len_indices: nat, CPS: nat, slot: nat, cIndex: nat)
+        requires TWO_UP_5 as nat <= len_indices 
+        requires CPS == max(1, min(MAX_COMMITTEES_PER_SLOT as nat, len_indices/ SLOTS_PER_EPOCH  as nat/ TARGET_COMMITTEE_SIZE as nat) as nat)
+        requires 0 <= slot < SLOTS_PER_EPOCH as nat// i.e. slot % SPE
+        requires 0 <= cIndex < CPS
+
+        ensures len_indices * ((slot * CPS + cIndex) + 1) / (CPS * SLOTS_PER_EPOCH as nat) > len_indices * (slot * CPS + cIndex) / (CPS * SLOTS_PER_EPOCH as nat);
+    {
+        natRatioRule(len_indices * ((slot * CPS + cIndex) + 1), len_indices * (slot * CPS + cIndex) , (CPS * SLOTS_PER_EPOCH as nat));
+
+        assert len_indices * ((slot * CPS + cIndex) + 1) - len_indices  * (slot * CPS + cIndex) >=  (CPS  * SLOTS_PER_EPOCH as nat) ==> 
+                len_indices * ((slot * CPS + cIndex) + 1) / (CPS  * SLOTS_PER_EPOCH as nat) > len_indices * (slot * CPS + cIndex) / (CPS * SLOTS_PER_EPOCH as nat);
+
+        calc {
+            len_indices * ((slot * CPS + cIndex) + 1) - len_indices * (slot * CPS + cIndex);
+            {natExpansion(len_indices as nat, (slot * CPS + cIndex));} len_indices * (slot * CPS + cIndex) + len_indices - len_indices * (slot * CPS + cIndex);
+            len_indices as nat;
+        }
+        assert len_indices == len_indices * ((slot * CPS + cIndex) + 1) - len_indices * (slot * CPS + cIndex);
+
+        assert len_indices >= (CPS * SLOTS_PER_EPOCH as nat) <==> len_indices * ((slot * CPS + cIndex) + 1) - len_indices * (slot * CPS + cIndex) >=  (CPS * SLOTS_PER_EPOCH as nat);
+
+        assert  TWO_UP_5 as nat <= len_indices 
+            ==> len_indices >= (CPS * SLOTS_PER_EPOCH as nat) 
+            ==> len_indices * ((slot * CPS + cIndex) + 1) / (CPS * SLOTS_PER_EPOCH as nat) > len_indices * (slot * CPS + cIndex) / (CPS * SLOTS_PER_EPOCH as nat);
+    }
+
+}
